\subsection{Elasticities of substitution}
\label{sec:elaSub3}

Allen-Uzawa elasticity of substitution
\citep[see][]{sato67} 

\begin{equation}
\sigma_{i,j} = \begin{cases} 
        (1 - \rho )^{-1}
        & \text{for } i = 1,2; \; j=3 \\ 
        & \\
        \dfrac{(1-\rho_1)^{-1} - (1-\rho)^{-1}}
        {\delta \left( \dfrac{y}{
        B_1^{-\frac{1}{\rho_1}}}\right)^{1+\rho}}+(1-\rho)^{-1}
        & \text{for } i=1; \; j=2 
   \end{cases}
\end{equation}  


Hicks-McFadden elasticity of substitution
\citep[see][]{sato67} 

\begin{equation}
\sigma_{i,j} = \begin{cases}
        \dfrac{\dfrac{1}{\theta_i} + \dfrac{1}{\theta_j}}
        {(1-\rho_1) \left( \dfrac{1}{\theta_i} - \dfrac{1}{\theta^*} \right)
        + (1-\rho_2) \left( \dfrac{1}{\theta_j} - \dfrac{1}{\theta} \right)
        + (1-\rho) \left( \dfrac{1}{\theta^*} - \dfrac{1}{\theta} \right) }
        & \text{for } i=1,2; \; j=3 \\ 
        & \\
        (1-\rho_1)^{-1}
        & \mbox{text } i=1; \; j=2 
   \end{cases}
\end{equation} 

with 
\begin{align}
& \theta^* = \delta
            B_1^{\frac{\rho}{\rho_1}} \cdot y^\rho \\
& \theta = (1-\delta) x_3^{-\rho} \cdot y^{\rho} \\
& \theta_1 = \delta \delta_1 x_1^{-\rho_1} 
            B_1^{-\frac{\rho_1 - \rho}{\rho_1}}
            \cdot y^{\rho} \\
& \theta_2 = \delta (1 - \delta_1) x_2^{-\rho_1} 
            B_1^{-\frac{\rho_1 - \rho}{\rho_1}}
            \cdot y^{\rho} \\
& \theta_3 = \theta
\end{align}
