\subsection{Elasticities of substitution}
\label{sec:elaSub4}

Allen-Uzawa elasticity of substitution
\citep[see][]{sato67} 

\begin{equation}
\sigma_{i,j} = \begin{cases} 
        (1 - \rho )^{-1}
        & \text{for } i=1,2; \; j=3,4 \\ 
        & \\
        \dfrac{ (1-\rho_1)^{-1} - (1-\rho)^{-1}}
        {\delta \left( \dfrac{y}{
        B_1^{-\frac{1}{\rho_1}}}\right)^{1+\rho}}+(1-\rho)^{-1}  
        & \text{for } i=1; \; j=2\\
        & \\
        \dfrac{ (1-\rho_2)^{-1} - (1-\rho)^{-1}}
        {(1-\delta) \left( \dfrac{y}{ 
        B_2^{-\frac{1}{\rho_2}}}\right)^{1+\rho}}+(1-\rho)^{-1}  
        & \text{for } i=3; \; j=4 
   \end{cases}
\end{equation}  


Hicks-McFadden elasticity of substitution
\citep[see][]{sato67} 

\begin{equation}
\sigma_{i,j} = \begin{cases} 
        \dfrac{\dfrac{1}{\theta_i} + \dfrac{1}{\theta_j}}
        {(1-\rho_1) \left( \dfrac{1}{\theta_i} - \dfrac{1}{\theta^*} \right)
        + (1-\rho_2) \left( \dfrac{1}{\theta_j} - \dfrac{1}{\theta} \right)
        + (1-\rho) \left( \dfrac{1}{\theta^*} - \dfrac{1}{\theta} \right) }
        & \text{for } i=1,2; \; j=3,4 \\ 
        & \\
        (1-\rho_1)^{-1}
        & \text{for } i=1; \; j=2 \\
        & \\
        (1-\rho_2)^{-1}
        & \text{for } i=3, \; j=4 
   \end{cases}
\end{equation} 

with 
\begin{align}
& \theta^* = \delta
            B_1^{\frac{\rho}{\rho_1}} \cdot y^\rho \\
& \theta = (1-\delta)
            B_2^{\frac{\rho}{\rho_2}} \cdot y^{\rho} \\
& \theta_1 = \delta \delta_1 x_1^{-\rho_1} 
            B_1^{-\frac{\rho_1 - \rho}{\rho_1}}
            \cdot y^{\rho} \\
& \theta_2 = \delta (1 - \delta_1) x_2^{-\rho_1} 
            B_1^{-\frac{\rho_1 - \rho}{\rho_1}}
            \cdot y^{\rho} \\
& \theta_3 = ( 1 - \delta ) \delta_2 x_3^{-\rho_2} 
            B_2^{-\frac{\rho_2 - \rho}{\rho_2}}
            \cdot y^{\rho} \\
& \theta_4 = ( 1 - \delta ) (1 - \delta_2) x_4^{-\rho_2} 
            B_2^{-\frac{\rho_2 - \rho}{\rho_2}}
            \cdot y^{\rho} 
\end{align}
